theories/FV.v
@@ -3,22 +3,29 @@ From LambdaST Require Import
 
 Definition set A := A -> Prop.
 
-Definition empty {A : Type} : set A := fun _ => False.
+Definition empty_set {A} : set A :=
+  fun _ => False.
 
-Definition singleton {A : Type} (x : A) : set A :=
-    fun y => x = y.
+Definition singleton_set {A} (x : A) : set A :=
+  fun y => x = y.
 
-Definition union {A : Type} (X Y : set A) : set A :=
-    fun x => X x \/ Y x.
+Definition set_union {A} (X Y : set A) : set A :=
+  fun x => X x \/ Y x.
 
-Definition intersection {A : Type} (X Y : set A) : set A :=
-    fun x => X x /\ Y x.
+Definition set_intersection {A} (X Y : set A) : set A :=
+  fun x => X x /\ Y x.
 
-Definition minus {A : Type} (X Y : set A) : set A :=
-    fun x => X x /\ ~(Y x).
+Definition set_minus {A} (X Y : set A) : set A :=
+  fun x => X x /\ ~(Y x).
 
-Definition disjoint {A : Type} (X Y : set A) : Prop :=
-    (forall x, X x -> ~(Y x)) /\ (forall x, Y x -> ~(X x)).
+Definition Disjoint {A} (X Y : set A) : Prop :=
+  (forall x, X x -> ~(Y x)) /\ (forall x, Y x -> ~(X x)).
 
-Class FV (A : Type) :=
-  { fv : A -> set ident }.
+(* Meant to be read with *currying* in mind: `Contains a b` = `(Contains a) b`, i.e. "b contains a" *)
+Definition Contains {T} (a b : set T) := forall x, a x -> b x.
+Arguments Contains/ {T} a b.
+
+Definition SetEq {T} (a b : set T) := forall x, a x <-> b x.
+Arguments SetEq/ {T} a b.
+
+Class FV (A : Type) := { fv : A -> set ident }.
